# 题解
###7-1
```
#include<iostream>
#include<cmath>
using namespace std;
int main()
{
	long long n,a,b,c,d=1;
	cin>>n;
	for (int i=0;i<n;i++)
	{
	cin>>a>>b>>c;
	while(b>0)
	{
		if(b%2==1)
		d=(d*a)%c;
		b/=2;
		a=(a*a)%c;
	}
	cout<<d<<endl;
	d=1;
}
}
```
### 7-2
```
#include<iostream>
using namespace std; 
int main()
{
	int n,m,a[41];
	a[1]=1;a[2]=2;a[0]=0;
	cin>>n;
	for (int j=3;j<=40;j++)
		{
			a[j]=a[j-1]+a[j-2]	;
		}
	for (int i=0;i<n;i++)
	{
		cin>>m;
		cout<<a[m-1]<<endl;
	}
    return 0;
}
```
### 7-3
```
#include <iostream>
#include<cstring>
using namespace std;
int a[10000001];
bool is[10000001];
int sum;
void f(int n)
{
   memset(is,1,sizeof(is));
   is[0]=0;is[1]=0;
    for(int i=2;i<=n;i++)
  {
        if(is[i])
        a[sum++]=i;
        for(int j=0;j<sum&&i*a[j]<=n;j++)
       {
            is[i*a[j]]=0;
            if(i%a[j]==0)
         break;
        }
    }
}
int main()
{
    int n;
    cin>>n;
    f(n);
    cout<<sum<<endl;
}
```
### 7-4
```
#include<iostream>
#include<cmath>
using namespace std;
int main()
{
	long long n,a,b,c,d=1;
	cin>>n;
	for (int i=0;i<n;i++)
	{
	cin>>a>>b>>c;
	while(b>0)
	{
		if(b%2==1)
		d=(d*a)%c;
		b/=2;
		a=(a*a)%c;
	}
	cout<<d<<endl;
	d=1;
}
}
```